Started into stack evaluation

02Stack/Stack.thy
@@ -2,5 +2,29 @@ theory Stack
 imports "../01Expression/Expression"
 begin
 
+datatype frame = 
+  SApp expr
+| SBind
+| SProj nat
+| SCase type "expr list"
+| SUnfold type
+| STyApp type
+
+datatype stack_direction = Eval | Return
+
+datatype stack_state = StackState stack_direction expr "frame list" "expr list"
+
+fun unstack :: "expr \<Rightarrow> frame list \<Rightarrow> expr list \<Rightarrow> expr" where
+  "unstack e [] h = e"
+| "unstack e (SApp e' # s) h = unstack (App e e') s h"
+| "unstack e (SBind # s) [] = undefined"
+| "unstack e (SBind # s) (e' # h) = unstack (Let e' e) s h"
+| "unstack e (SProj l # s) h = unstack (Proj e l) s h"
+| "unstack e (SCase t cs # s) h = unstack (Case e t cs) s h"
+| "unstack e (SUnfold t # s) h = unstack (Unfold t e) s h"
+| "unstack e (STyApp t # s) h = unstack (TyApp e t) s h"
+
+primrec unstack_state :: "stack_state \<Rightarrow> expr" where
+  "unstack_state (StackState _ e s h) = unstack e s h"
 
 end
